src/named/Matches.v
@@ -9,7 +9,7 @@ Import ListNotations.
 Open Scope string.
 Open Scope list.
 From Utils Require Import Utils.
-From Named Require Import Core.
+From Named Require Import Core Elab.
 Import Core.Notations.
 Import OptionMonad.
 
@@ -261,248 +261,361 @@ Goal
   vm_compute; exact I.
 Qed.
 
-(*
-Variant matchable := match_exp (e:exp) | match_sort (s : sort).
 
-Coercion match_exp : exp >-> matchable.
-Coercion match_sort : sort >-> matchable.
-
-(* matching checks only work when the pattern contains all 
-   variables in args. This allows us to use multiple patterns
-   to cover the variables, such as for an equivalence rule
+(*TODO: move to matches or new parstep file*)
+(*If the LHS of a term eq rule directly applies to e, 
+  return the rule name and s such that LHS[/s/] = e.
+  Rules are scanned from the root of the language.
  *)
-Fixpoint match_all_unordered (l_exp l_pat : list matchable): option subst :=
-  match l_exp, l_pat with
-  | [], [] => do ret []
-  | (match_exp e)::l'_exp, (match_exp pat)::l'_pat =>
-    do s <- matches_unordered e pat;
-       s' <- match_all_unordered l'_exp l'_pat;
-       ret (unordered_merge_unsafe s s')
-  | (match_sort e)::l'_exp, (match_sort pat)::l'_pat =>
-    do s <- matches_unordered_sort e pat;
-       s' <- match_all_unordered l'_exp l'_pat;
-       ret (unordered_merge_unsafe s s')
-  | _, _ => None
+Import OptionMonad.
+
+Inductive step_instruction :=
+| cong_instr : list step_instruction -> step_instruction
+| refl_instr : step_instruction
+| redex_instr : string -> ctx -> sort -> exp -> exp -> subst -> step_instruction.
+
+Fixpoint step_redex_term (l : lang) (e : exp) : option step_instruction :=
+  match l with
+  | [] => None
+  | (n,term_eq_rule c e1 e2 t')::l' =>
+    match step_redex_term l' e with
+    | Some e' => Some e'
+    | None => do s <- matches e e1 (map fst c);
+              ret (redex_instr n c t' e1 e2 s)
+    end
+  | _::l' => step_redex_term l' e
   end.
 
-Fixpoint check_all (l_exp l_pat : list matchable) s :=
-  match l_exp, l_pat with
-  | [],[] => true
-  | (match_exp e)::l'_exp, (match_exp pat)::l'_pat =>
-    (e == pat[/s/]) && (check_all l'_exp l'_pat s)
-  | (match_sort e)::l'_exp, (match_sort pat)::l'_pat =>
-    (e == pat[/s/]) && (check_all l'_exp l'_pat s)
-  | _, _ => false
-end.
 
-Definition match_all l_exp l_pat args :=
-  do s <- match_all_unordered l_exp l_pat;
-     s' <- order_subst s args;
-     (* this condition can fail because merge doesn't check for conflicts *)
-     !check_all l_exp l_pat s';
-     ret s'.
+Inductive wf_term_no_conv l : ctx -> exp -> sort -> Prop :=
+  | wf_term_by_no_conv : forall c n s args c' t,
+      In (n, term_rule c' args t) l ->
+      wf_args l c s c' ->
+      wf_term_no_conv l c (con n s) t[/(with_names_from c' s)/]
+  | wf_term_var_no_conv : forall c n t,
+      In (n, t) c ->
+      wf_term_no_conv l c (var n) t.
+Local Hint Constructors wf_term_no_conv : lang_core.
 
-Definition matchable_related s (e p : matchable) : Prop :=
-  match e, p with
-  | match_exp e', match_exp p' => e' = p'[/s/]
-  | match_sort e', match_sort p' => e' = p'[/s/]
-  | _,_ => False
+Lemma wf_term_peel_convs l c e t
+  : wf_term l c e t -> exists t', wf_term_no_conv l c e t'.
+Proof.
+  induction 1; basic_core_crush.
+Qed.
+
+
+
+
+Fixpoint step_term l e : option step_instruction :=
+  match step_redex_term l e with
+  | Some i => Some i
+  | None =>
+    match e with
+    | var x => Some refl_instr
+    | con n s =>
+      option_map cong_instr (Mmap (step_term l) s)
+    end
   end.
 
-Arguments matchable_related s !e !p/.
 
-Lemma check_all_related l lp s
-  : check_all l lp s -> List.Forall2 (matchable_related s) l lp.
+Require Import Ltac2.Ltac2.
+Import Ltac2.Message Ltac2.Control.
+Set Default Proof Mode "Classic".
+
+Lemma wf_args_cons2
+     : forall (l : lang) (c : ctx) (s : list exp) (c' : named_list sort) 
+         (name name': string) (e e': exp) (t t' : sort),
+       wf_term l c e t [/with_names_from c' s /] ->
+       wf_term l c e' t' [/with_names_from ((name,t)::c') (e::s) /] ->
+       wf_args l c s c' -> wf_args l c (e'::e :: s) ((name',t')::(name, t) :: c').
 Proof.
-  revert lp; induction l; intro lp; destruct lp; intros; simpl in *;
-    ltac1:(repeat match goal with
-                  | h : matchable |- _=> destruct h
-                  | [h : is_true false |- _] => inversion H
-                  | [|- _ = _] => apply /eqP; assumption
-                  | [|-_ ]=> break; try (constructor; simpl); auto
-                  end).
+  eauto with lang_core.
 Qed.
 
-Lemma match_all_recognizes l lp args s
-  : match_all l lp args = Some s -> List.Forall2 (matchable_related s) l lp.      
+Lemma eq_args_cons2
+     : forall (l : lang) (c : ctx) (s1 s2 : list exp) (c' : named_list sort) 
+         (name name': string) (e1 e2 e1' e2': exp) (t t' : sort),
+       eq_args l c c' s1 s2 ->
+       eq_term l c t [/with_names_from c' s2 /] e1 e2 ->
+       eq_term l c t' [/with_names_from ((name,t)::c') (e2::s2) /] e1' e2'->
+       eq_args l c ((name',t')::(name, t) :: c') (e1'::e1 :: s1) (e2'::e2 :: s2) .
 Proof.
-  intro H.
-  apply check_all_related.
-  revert H.
-  unfold match_all.
-  repeat ltac1:(case_match;[|inversion]).
-  intro seq; inversion seq; clear seq; subst.
-  rewrite <-HeqH1.
-  reflexivity.
+  eauto with lang_core.
 Qed.
 
-
-Lemma match_all_args e pat args s
-  : match_all e pat args = Some s ->
-    args = map fst s.
-Proof.
-  unfold match_all.
-  repeat ltac1:(case_match;[|inversion]).
-  ltac1:(inversion); subst.
-  eapply order_subst_args.
-  symmetry; eauto.
-Qed.
-
-(* Designed for the specific case of generating
-   a pair of (potentially) related substitutions *)
-Definition match_all_le l1 lp1 l2 lp2 args : option (subst* subst) :=
-  do s1 <- match_all_unordered l1 lp1;
-     s2 <- match_all_unordered l2 lp2;
-     s1'' <- order_subst (unordered_merge_unsafe s2 s1) args;
-     s2'' <- order_subst (unordered_merge_unsafe s1 s2) args;
-     (* this condition can fail because merge doesn't check for conflicts *)
-     !check_all l1 lp1 s1'';
-     (* this condition can fail because merge doesn't check for conflicts *)
-     !check_all l2 lp2 s2'';
-     ret (s1'',s2'').
-
-Lemma match_all_le_recognizes_l l1 lp1 l2 lp2 args s1 s2
-  : match_all_le l1 lp1 l2 lp2 args = Some (s1,s2) ->
-    List.Forall2 (matchable_related s1) l1 lp1.      
-Proof.
-  intro H.
-  apply check_all_related.
-  revert H.
-  unfold match_all_le.
-  repeat ltac1:(case_match;[|inversion]).
-  intro seq; inversion seq; clear seq; subst.
-  rewrite <-HeqH3.
-  reflexivity.
-Qed.
-
-
-Lemma match_all_le_recognizes_r l1 lp1 l2 lp2 args s1 s2
-  : match_all_le l1 lp1 l2 lp2 args = Some (s1,s2) ->
-    List.Forall2 (matchable_related s2) l2 lp2.      
-Proof.
-  intro H.
-  apply check_all_related.
-  revert H.
-  unfold match_all_le.
-  repeat ltac1:(case_match;[|inversion]).
-  intro seq; inversion seq; clear seq; subst.
-  rewrite <-HeqH4.
-  reflexivity.
-Qed.
-
-
-Lemma match_all_le_args_l l1 lp1 l2 lp2 args s1 s2
-  : match_all_le l1 lp1 l2 lp2 args = Some (s1,s2) ->
-    args = map fst s1.
-Proof.
-  unfold match_all_le.
-  repeat ltac1:(case_match;[|inversion]).
-  ltac1:(inversion); subst.
-  eapply order_subst_args.
-  symmetry; eauto.
-Qed.
-
-
-Lemma match_all_le_args_r l1 lp1 l2 lp2 args s1 s2
-  : match_all_le l1 lp1 l2 lp2 args = Some (s1,s2) ->
-    args = map fst s2.
-Proof.
-  unfold match_all_le.
-  repeat ltac1:(case_match;[|inversion]).
-  ltac1:(inversion); subst.
-  eapply order_subst_args.
-  symmetry; eauto.
-Qed.
-
-Definition apply_le_term l n (e1 e2 : exp) (t : sort) : option (subst * subst*ctx) :=
-  do (term_le c pat1 pat2 patt) <- named_list_lookup_err l n;
-  (s1,s2) <- match_all_le [ e1:matchable]
-                          [ pat1 : matchable]
-                          [ t:matchable; e2:matchable]
-                          [ patt:matchable; pat2:matchable]
-                          (map fst c);
-  ret (s1,s2,c).
-
-Lemma apply_le_term_recognizes n l c e1 e2 t s1 s2 c'
+Lemma eq_term_by_with_subst name l c c' e1 e2 t s 
   : wf_lang l ->
-    apply_le_term l n e1 e2 t = Some (s1,s2,c') ->
-    le_subst l c c' s1 s2 ->
-    le_term l c t e1 e2.
-(* e1 = e1'[/s1/]
-   e2 = e2'[/s2/]
-   e1' ~ e2' (by rule n)*)
+    In (name, term_eq_rule c' e1 e2 t) l ->
+    wf_subst l c s c' ->
+    eq_term l c t[/s/] e1[/s/] e2[/s/].
 Proof.
-  intro wfl.
-  unfold apply_le_term.
-  repeat ltac1:(case_match;[|inversion]).
-  destruct r; 
-    repeat ltac1:(case_match;[|inversion]);
-    try ltac1:(by inversion).
-  ltac1:(break); simpl.
-  intro seq; inversion seq; clear seq; subst.
-  
-  pose HeqH0.
-  symmetry in e3.
-  apply match_all_le_recognizes_l in e3.
-  inversion e3; subst.
-  clear e3 H4.
-  
-  pose HeqH0.
-  symmetry in e3.
-  apply match_all_le_recognizes_r in e3.
-  inversion e3; inversion H5; subst.
-  clear e3 H5 H11.
-
-  simpl in *; subst.
-  intro.
-  apply (@named_list_lookup_err_in rule_eqType) in HeqH.  
-  eapply le_term_subst; eauto.
-  eapply rule_in_wf in HeqH; auto; inversion HeqH; subst; assumption.
-  eapply le_term_by; eauto.
+  intros.
+  eapply eq_term_subst; [| eapply eq_subst_refl; eassumption
+                         | eapply eq_term_by; eassumption].
+  with_rule_in_wf_crush.
 Qed.
 
-Arguments apply_le_term_recognizes n%string_scope [l c e1 e2 t s1 s2 c'].
 
-(*
-Goal match_all_unordered
-            [ Exp.con "ty_subst"
-                  [ Exp.var "A"; Exp.con "id" [ Exp.var "G"]; Exp.var "G"; Exp.var "G"]:matchable]
-            [ Exp.con "ty_subst"
-                [ Exp.var "A"; Exp.con "id" [ Exp.var "G"]; Exp.var "G"; Exp.var "G"]:matchable].
-Proof.
-  unfold match_all_unordered.
-  ltac1:(case_match).
-  unfold matches_unordered in HeqH.
-  cbv [exp_depth foldl Nat.max] in HeqH.
-  unfold matches_unordered_fuel in HeqH.
-  
-  vm_compute in HeqH.
+Ltac solve_in := apply named_list_lookup_err_in; compute; reflexivity.
+
+Ltac lookup_wf_lang := assumption (*TODO: add to ctx beforehand, use assumption here*).
 
 
+(*TODO: adapt to work w/ possible evars in r?*)
+Ltac solve_named_list_in_from_value :=
+  match goal with
+    [|- In ?p ?l] =>
+    let x := eval simpl in (In p l) in
+        match x with
+        | context [(?n, ?r) = (?n', ?r)] =>
+          assert (n = n') by reflexivity
+        end;
+                           apply named_list_lookup_err_in; compute; reflexivity
+  end.
+
+Ltac is_term_rule := eapply eq_term_by; solve_named_list_in_from_value.
+
+Ltac solve_len_eq := solve[ repeat constructor].
+
+Ltac term_cong :=
+  eapply term_con_congruence;
+  [ solve_in
+  | solve_len_eq
+  | compute; reflexivity
+  | lookup_wf_lang
+  | repeat match goal with [|- eq_args _ _ _ _ _] =>
+                           simple apply eq_args_nil
+                           || simple eapply eq_args_cons2
+                           || simple eapply eq_args_cons
+           end].
+Ltac term_refl := 
+  apply eq_term_refl; shelve (*TODO: solve[repeat t']*).
 
 
+Ltac eq_term_by s := 
+  eapply (eq_term_by _ _ s); solve_in.
 
-
-e1 ~ e2
-<= e1 = e1'[/s1/]
-   e2 = e2'[/s2/]
-   e1' ~ e2' (by rule n)
-
-args : t...
---------- n
-e1' ~ e2'
-
-s1 = s2
-
-beta: C |- (\x.e) e'~ e[e'/x]
-
-           ....
----- refl  -------
-4~4        4~2+2
-----------------------cong
-(4,4) ~ (2+2,4)
------------------- beta
-(\x.(x,x)) 4 ~ (2+2,4)
-
+(*TODO: optimize where this is used so that I don't
+  duplicate work?
 *)
+Local Ltac t' :=
+  match goal with
+  | [|- fresh _ _ ]=> apply use_compute_fresh; compute; reflexivity
+  | [|- sublist _ _ ]=> apply (use_compute_sublist string_dec); compute; reflexivity
+  | [|- In _ _ ]=> solve_in
+  | [|- wf_term _ _ _ _] => assumption || eapply wf_term_var || eapply wf_term_by'
+  | [|-wf_args _ _ _ _] => simple apply wf_args_nil
+                           || simple eapply wf_args_cons2
+                           || simple eapply wf_args_cons
+  | [|-wf_subst _ _ _ _] => constructor
+  | [|-wf_ctx _ _] => assumption || constructor
+  | [|- wf_sort _ _ _] => eapply wf_sort_by
+  | [|- wf_lang _] => lookup_wf_lang
+  | [|- _ = _] => compute; reflexivity
+  end.
+
+  Local Ltac t :=
+  match goal with
+  | [|- fresh _ _ ]=> apply use_compute_fresh; compute; reflexivity
+  | [|- sublist _ _ ]=> apply (use_compute_sublist string_dec); compute; reflexivity
+  | [|- In _ _ ]=> apply named_list_lookup_err_in; compute; reflexivity
+  | [|- len_eq _ _] => econstructor
+  | [|-elab_sort _ _ _ _] => eapply elab_sort_by
+  | [|-elab_ctx _ _ _] => econstructor
+  | [|-elab_args _ _ _ _ _ _] => eapply elab_args_cons_ex' || econstructor
+  | [|-elab_term _ _ _ _ _] => eapply elab_term_var || eapply elab_term_by'
+  | [|-wf_term _ _ _ _] => shelve
+  | [|-elab_rule _ _ _] => econstructor
+  | [|- _ = _] => compute; reflexivity
+  end.
+
+    
+    (*TODO: only works if all variables appear on the lhs*)
+    Ltac redex_steps_with lang name :=
+    let mr := eval compute in (named_list_lookup_err lang name) in
+    lazymatch mr with
+    | Some (term_eq_rule ?c ?e1p ?e2p ?tp) =>
+      lazymatch goal with
+      | [|- eq_term ?l ?c' ?t ?e1 ?e2] =>
+        let ms := eval compute in (matches e1 e1p (map fst c)) in
+            lazymatch ms with
+            | Some ?s =>
+              replace (eq_term l c' t e1 e2)
+                with (eq_term l c' tp[/s/] e1p[/s/] e2p[/s/]);
+                [| reflexivity];
+                eapply eq_term_subst;
+                [| | eq_term_by name];
+                [solve [repeat t']|apply eq_subst_refl; solve [repeat t']]
+            | None => fail "lhs" e1 "does not match rule" e1p
+            end
+      | _ => fail "Goal not a term equality"
+      end
+    | _ => fail "Rule not found"
+    end.
+
+    Ltac2 step_redex name c' tp e1p e2p s :=
+        lazy_match! goal with
+        | [|- eq_term ?l ?c _ _ _] =>
+          assert (eq_term $l $c $tp[/$s/] $e1p[/$s/] $e2p[/$s/])> [| ltac1:(eassumption)];
+          apply (@eq_term_by_with_subst $name $l $c $c' $e1p $e2p $tp $s); solve [repeat ltac1:(t')]
+        end.
+
+    Ltac2 get_goal_lang () :=
+      lazy_match! goal with
+      |[|- eq_term ?l _ _ _ _ ] => l
+      end.
+
+    Ltac2 rec step_by_instructions i :=
+      lazy_match! i with
+      | refl_instr => ltac1:(term_refl)
+      | cong_instr ?s =>
+        (*have to run this before term_cong because for some reason
+          it expects a focussed goal
+         *)
+        let s_tac_list := List.rev (step_all_instructions s) in
+        ltac1:(term_cong);
+        Control.dispatch s_tac_list
+      | redex_instr ?name ?c' ?tp ?e1p ?e2p ?s =>
+        step_redex name c' tp e1p e2p s
+      | _ => backtrack_tactic_failure "input not an evaluated instruction"
+    end
+    with step_all_instructions s :=
+      lazy_match! s with
+      | [] => []
+      | ?i::?s' => (fun () => step_by_instructions i)::(step_all_instructions s')
+      | _ => backtrack_tactic_failure "input not an evaluated list"
+      end.
+
+    Ltac2 get_step_instructions () :=
+    lazy_match! goal with
+     | [|- eq_term ?l ?c' ?t ?e1 ?e2] =>
+       let mi := Std.eval_vm None constr:(step_term $l $e1) in
+       lazy_match! mi with
+       | Some ?i => i
+       | None =>  backtrack_tactic_failure "could not generate step instructions"
+       end
+     | [|-_] => backtrack_tactic_failure "goal not a term equality"
+  end.
+      
+    Ltac2 step () :=
+      step_by_instructions (get_step_instructions ()).
+    Ltac2 print_steps () :=
+      print (of_constr (get_step_instructions())).
+
+  Ltac compute_eq_compilation :=
+    match goal with
+    |[|- eq_sort ?l ?ctx ?t1 ?t2] =>
+     let ctx' := eval compute in ctx in
+     let t1' := eval compute in t1 in
+     let t2' := eval compute in t2 in
+     change (eq_sort l ctx' t1' t2')
+    |[|- eq_term ?l ?ctx ?e1 ?e2 ?t] =>
+     let ctx' := eval compute in ctx in
+     let e1' := eval compute in e1 in
+     let e2' := eval compute in e2 in
+     let t' := eval compute in t in
+     change (eq_term l ctx' e1' e2' t')
+    end.
+
+    
+    Ltac reduce :=
+      repeat (eapply eq_term_trans; [ltac2:(step())|compute_eq_compilation]);
+      term_refl.
+    Ltac by_reduction :=
+      eapply eq_term_trans; [reduce | eapply eq_term_sym; reduce].
+
+
+
+
+
+
+(* TODO: something like this is necessary for
+   a reflective stepper. 
+   The only other option is for the stepper to
+   out put a list of side-conditions
+
+Lemma subst_wf_injective l c s
+  : wf_lang l ->
+    all_fresh s ->
+    (forall c' t',
+        wf_sort l c' t' ->
+          wf_sort l c t'[/s/] ->
+          set_eq (map fst s) (fv_sort t') ->
+          map fst s = map fst c' ->
+          wf_subst l c s c') /\
+    (forall c' e' t',
+        wf_term l c' e' t' ->
+        forall t,
+          wf_term l c e'[/s/] t ->
+          set_eq (map fst s) (fv e') ->
+          map fst s = map fst c' ->
+          (*wf_term l c e  t'[/s/] /\*)  wf_subst l c s c') /\
+    (forall c' s1 c1,
+        wf_args l c' s1 c1 ->
+        forall c2,
+          wf_args l c s1[/s/] c2 ->
+          set_eq (map fst s) (fv_args s1) ->
+          map fst s = map fst c' ->
+          wf_subst l c s c').
+Proof.
+  intros wfl allfs.
+  apply wf_judge_ind.
+  {
+    intro_to wf_sort.
+    inversion 1; basic_goal_prep;
+      basic_core_crush.
+  }
+  (*
+    pose proof (in_all_fresh_same _ _ _ _ (wf_lang_all_fresh wfl) H H6).
+    basic_core_crush. *)
+  {
+    intro_to wf_term.
+    intro wft.
+    apply wf_term_peel_convs in wft.
+    destruct wft as [t' wft].
+    safe_invert wft.
+    basic_goal_prep.
+    pose proof (in_all_fresh_same _ _ _ _ (wf_lang_all_fresh wfl)  H H5).
+    safe_invert H4; eauto.
+  }
+  {
+    firstorder.
+  }
+  {
+    destruct s; basic_goal_prep.
+    {
+      destruct c0; basic_goal_prep;
+        basic_utils_crush.
+    }
+    {
+      assert (s=[]) by 
+          admit (*incl and all_fresh*).
+      subst; basic_goal_prep.
+      assert (s0 = n) by admit (*set_eq*).
+      subst.
+      rewrite eqb_refl in H0.
+      destruct c0; basic_goal_prep.
+      basic_utils_crush.
+      safe_invert H2; subst.
+      destruct c0; basic_goal_prep.
+      2:basic_utils_crush.
+      constructor.
+      constructor.
+      
+      admit (*incl and all_fresh*).
+    basic_core_crush.
+    destruct s; basic_goal_prep;
+      basic_core_crush.
+    destruct c0; basic_goal_prep;
+      basic_utils_crush.
+    destruct c0; basic_goal_prep;
+      basic_core_crush.
+    
+    
+    
+    exfalso.
+    clear H2 H5 H4 H0 H t t0 c0.
+    unfold incl in *
+    simpl in
+    todo: list-set math
 *)
