src/named/Subst.v
@@ -1,24 +1,20 @@
-Require Import mathcomp.ssreflect.all_ssreflect.
 Set Implicit Arguments.
-Unset Strict Implicit.
-Unset Printing Implicit Defensive.
 Set Bullet Behavior "Strict Subproofs".
 
-
-From Ltac2 Require Import Ltac2.
-From Utils Require Import Utils Monad.
-From Named Require Import Exp ARule ImCore Pf Interactive.
-Import Exp.Notations ARule.Notations.
-Require Import String.
-
+Require Import String List.
+Import ListNotations.
+Open Scope string.
+Open Scope list.
+From Utils Require Import Utils.
+From Named Require Import Core Elab.
+Import Core.Notations.
 
 Require Coq.derive.Derive.
 
-Set Default Proof Mode "Ltac2".
 
 (* syntax of categories *)
 Definition cat_lang : lang :=
-  [::
+  [
      [:> "G1" : #"env",
          "G2" : #"env",
          "G3" : #"env",
@@ -57,503 +53,20 @@ Definition cat_lang : lang :=
   ]
   ]%arule.
 
-Set Default Proof Mode "Classic".
-
-(*TODO: move somewhere? need to deal w/ cat_lang *)
-Ltac nth_tail_show_hd :=
-  erewrite nth_tail_show_hd;[cbn[nth cat_lang]| by compute].
-
-
-Ltac store_bound_comp_as Hcmp :=
-  match goal with
-    [|- context ctx [Mbind ?f ?comp] ]=>
-    let cmp := fresh "comp" in
-    remember comp as cmp eqn:Hcmp;
-    let comp' := eval hnf in comp in
-    change (cmp = comp') in Hcmp
-  end.
-
-
-Ltac store_bound_comp_as_in Hcmp H :=
-  match type of H with
-    context ctx [Mbind ?f ?comp]=>
-    let cmp := fresh "comp" in
-    remember comp as cmp eqn:Hcmp in H;
-    let comp' := eval hnf in comp in
-    change (cmp = comp') in Hcmp
-  end.
-
-Fixpoint noim_elab l (e : interactive PfGoal lang) : interactive PfGoal lang :=
-  match e  with
-  | iret el => iret el
-  | itau i => noim_elab l i
-  | ifail => ifail
-  | iask _ (expand_sort_args (scon n s)) k =>
-    do (sort_rule c' args) <?- lift (named_list_lookup_err l n);
-    res <- if size args == size c' then noim_elab l (k s)
-           else iask (expand_sort_args (scon n s)) (fun a => noim_elab l (k a));
-       ret res
-  | iask _ (expand_term_args (con n s) t) k =>
-    do (sort_rule c' args) <?- lift (named_list_lookup_err l n);
-    res <- if size args == size c' then noim_elab l (k s)
-           else iask (expand_term_args (con n s) t) (fun a => noim_elab l (k a));
-       ret res                                                          
-  | iask _ d k => iask d (fun a => noim_elab l (k a))
-  end.
 
     
-Derive cat_lang_pf
-       SuchThat (find_lang_pf_with cat_lang_pf cat_lang handle_refls)
-       As cat_lang_pf_ok.
+Derive cat_lang_elab
+       SuchThat (elab_lang cat_lang cat_lang_elab)
+       As cat_lang_wf.
 Proof.
-  exists (fun l => noim_elab l (default_lang_elaborator 100 l)).
-  enter_interactive 100.
-  coerce_input_to_cons tl.
-  remember (noim_elab cat_lang (default_lang_elaborator 100 cat_lang)) as el.
-  remember (default_lang_elaborator 100 cat_lang) as el' in Heqel.
-  match goal with
-    [ H : el' = ?e|-_] =>
-    let x := eval hnf in e in
-        change (el' = x) in H
-  end.
-  rewrite Heqel' in Heqel.
-  clear Heqel'.
-  cbn [noim_elab cat_lang] in Heqel.
-  cbn [lift named_list_lookup_err cat_lang String.eqb Ascii.eqb Bool.eqb fst snd] in Heqel.
-  cbn beta match delta [Mbind ibind Mret interactive_monad] in Heqel.
-  match goal with
-    [|- ?m = ?r /\ ?p] =>
-    let x := eval vm_compute in m in
-        change (x = r /\ p)
-  end.
-  cbn [handle_from_list nth].
-  match goal with
-    [ |- context ctx[_ ?f (iret ?a)] ]=>
-      let x := context ctx [f a]in change x
-  end.
-  match goal with
-    [|- ?m = ?r /\ ?p] =>
-    let x := eval hnf in m in
-        change (x = r /\ p)
-  end.
-  fold ibind.
-  hnf_elaborator
-  
-
-Lemma cat_lang_ok : find_wf_lang_elaboration cat_lang.
-Proof.
-  unfold find_wf_lang_elaboration.
-  enter_interactive.
-  rewrite <-(@nth_tail_0 _ cat_lang) at 1.
-  nth_tail_show_hd.
-  repeat process_interactive.
-  {
-    instantiate_term hd (pcon "env" [::]).
-    vm_compute.
-    reflexivity.
-  }
-  repeat process_interactive.
-  {
-    instantiate_term hd0 (pcon "env" [::]).
-    vm_compute.
-    reflexivity.
-  }
-  {
-    instantiate_term hd1 (pcon "env" [::]).
-    vm_compute.
-    reflexivity.
-  }
-  repeat process_interactive.
-  {
-    instantiate_term hd2 (pcon "env" [::]).
-    vm_compute.
-    reflexivity.
-  }
-  {
-    instantiate_term hd3 (pcon "env" [::]).
-    vm_compute.
-    reflexivity.
-  }
-  repeat process_interactive.
-  {
-    instantiate_term hd4 (pcon "env" [::]).
-    vm_compute.
-    reflexivity.
-  }
-  { instantiate_term hd5 (pvar "G1").
-    vm_compute; eauto.
-  }    
-  repeat process_interactive.
-  {
-    instantiate_term hd6 (pvar "G2").
-    vm_compute; eauto.
-  }    
-  repeat process_interactive.
-  {
-    instantiate_term hd7 (pvar "G4").
-    vm_compute; eauto.
-  }    
-  repeat process_interactive.
-  {
-    instantiate_term hd8 (pcon "sub" [:: pvar "G2"; pvar "G1"]).
-    vm_compute.
-    reflexivity.
-  }
-  repeat process_interactive.
-  
-  {
-    instantiate_term hd9 (pvar "G2").
-    vm_compute; eauto.
-  }    
-  repeat process_interactive.
-  {
-    instantiate_term hd10 (pvar "G3").
-    vm_compute; eauto.
-  }    
-  repeat process_interactive.
-  {
-    instantiate_term hd11 (pvar "G4").
-    vm_compute; eauto.
-  }    
-  repeat process_interactive.
-  {
-    instantiate_term hd12 (pcon "sub" [:: pvar "G3"; pvar "G2"]).
-    vm_compute.
-    reflexivity.
-  }
-  repeat process_interactive.
-  {
-    instantiate_term hd13 (pcon "sub" [:: pvar "G4"; pvar "G3"]).
-    vm_compute.
-    reflexivity.
-  }
-  repeat process_interactive.
-  {
-    instantiate_term hd14 (pcon "sub" [:: pvar "G4"; pvar "G2"]).
-    vm_compute.
-    reflexivity.
-  }
-  repeat process_interactive.
-  {
-    instantiate_term hd15 (pcon "sub" [:: pvar "G4"; pvar "G1"]).
-    vm_compute.
-    reflexivity.
-  }
-  {
-    instantiate_term hd16 (pvar "G1").
-    vm_compute.
-    eauto.
-  }
-  repeat process_interactive.
-  {
-    instantiate_term hd17 (pvar "G3").
-    vm_compute.
-    eauto.
-  }
-  repeat process_interactive.
-  {
-    instantiate_term hd18 (pvar "G4").
-    vm_compute.
-    eauto.
-  }
-  repeat process_interactive.
-  {
-    instantiate_term hd19 (pvar "G1").
-    vm_compute.
-    eauto.
-  }
-  repeat process_interactive.
-  {
-    instantiate_term hd20 (pvar "G2").
-    vm_compute.
-    eauto.
-  }
-  repeat process_interactive.
-  {
-    instantiate_term hd21 (pvar "G3").
-    vm_compute.
-    eauto.
-  }
-  repeat process_interactive.
-  {
-    instantiate_term hd22 (pcon "sub" [:: pvar "G2"; pvar "G1"]).
-    vm_compute.
-    reflexivity.
-  }
-  repeat process_interactive.
-  {
-    instantiate_term hd23 (pcon "sub" [:: pvar "G3"; pvar "G2"]).
-    vm_compute.
-    reflexivity.
-  }
-  repeat process_interactive.
-  {
-    instantiate_term hd24 (pcon "sub" [:: pvar "G3"; pvar "G1"]).
-    vm_compute.
-    reflexivity.
-  }
-  repeat process_interactive.
-  {
-    instantiate_term hd25 (pcon "sub" [:: pvar "G4"; pvar "G3"]).
-    vm_compute.
-    reflexivity.
-  }
-  repeat process_interactive.
-  {
-    instantiate_term hd26 (pcon "sub" [:: pvar "G4"; pvar "G1"]).
-    vm_compute.
-    reflexivity.
-  }
-  repeat process_interactive.
-  {
-    instantiate_term hd27 (pcon "env" [::]).
-    vm_compute.
-    reflexivity.
-  }
-  repeat process_interactive.
-  {
-    instantiate_term hd28 (pcon "env" [::]).
-    vm_compute.
-    reflexivity.
-  }
-  {
-    instantiate_term hd29 (pcon "env" [::]).
-    vm_compute.
-    reflexivity.
-  }
-  repeat process_interactive.
-  {
-    instantiate_term hd30 (pcon "env" [::]).
-    vm_compute.
-    reflexivity.
-  }
-  repeat process_interactive.
-  {
-    instantiate_term hd31 (pvar "G").
-    vm_compute.
-    eexists; reflexivity.
-  }
-  repeat process_interactive.
-  {
-    instantiate_term hd32 (pvar "G").
-    vm_compute.
-    eauto.
-  }
-  repeat process_interactive.
-  {
-    instantiate_term hd33 (pvar "G'").
-    vm_compute.
-    eauto.
-  }
-  repeat process_interactive.
-  {
-    instantiate_term hd32 (pvar "G").
-    vm_compute.
-    eauto.
-  }
-    cbn.
-  process_interactive.
-  process_interactive.
-  process_interactive.
-  rewrite Mbind_assoc.
-  
-  process_interactive.
-  rewrite Mbind_assoc.
-  process_interactive.
-  rewrite Mbind_assoc.
-  rewrite Mbind_assoc.
-  lazymatch goal with
-   | [|- context ctx [focus ?comp] ]=>
-     let comp' := eval hnf in comp in
-         idtac comp' end.
-         lazymatch comp' with
-         | Mbind ?g (Mbind ?f ?cmp) ?tl =>
-           idtac f
-         end
-  end.
-  
-  process_interactive.
-  lazymatch goal with
-  | [|- context out_ctx
-                [Mbind ?f ?cmp ?tl] ]=>
-    lazymatch cmp with
-      context in_ctx [focus ?a] =>
-      lazymatch type of tl with
-      | list ?Q =>
-      let hd := fresh "hd" in evar (hd : Q);
-    let tl' := fresh "tl" in evar (tl' : list Q);
-    instantiate_term tl (hd::tl')
-      end
-    end
-  end.
-  let x := context ctx [focus (f a)] in
-      change x
-  store_bound_comp_as Hcmp.
-  store_bound_comp_as_in Hcmp0 Hcmp.
-  store_bound_comp_as_in Hcmp1 Hcmp0.
-  store_bound_comp_as_in Hcmp2 Hcmp1.
-  rewrite Hcmp2 in Hcmp1.
-  clear Hcmp2.
-  rewrite monad_bind_ret in Hcmp1.
-  store_bound_comp_as_in Hcmp2 Hcmp1.
-  store_bound_comp_as_in Hcmp3 Hcmp2.
-  rewrite monad_bind_ret in Hcmp3.
-  pose (p := Mbind
-            (fun s : seq exp =>
-             Mbind (fun pe : pf => do ret [:: pe])
-               (elab_term (nth_tail 1 cat_lang)
-                  {{c"G1" : #"env",
-                     "G2" : #"env",
-                     "G3" : #"env",
-                     "G4" : #"env",
-                     "f" : #"sub" %"G1" %"G2",
-                     "g" : #"sub" %"G2" %"G3"}} {{e%"G3"}}
-                  {{s#"env"}} [/with_names_from (@nil (string *exp)) s /]))
-            (lift
-               (synth_wf_args (synth_wf_term (nth_tail 1 cat_lang)) [::]
-                  {{c"G1" : #"env",
-                     "G2" : #"env",
-                     "G3" : #"env",
-                     "G4" : #"env",
-                     "f" : #"sub" %"G1" %"G2",
-                     "g" : #"sub" %"G2" %"G3"}} {{c }}))).
-  let x := eval hnf in p in idtac x.
-  store_bound_comp_as_in Hcmp4 Hcmp3.
-  rewrite Hcmp2 in Hcmp1.
-  clear Hcmp2.
-  rewrite monad_bind_ret in Hcmp1.
-  
-  Transparent elab_lang.
-  hnf.
-  unfold elab_lang.
-  store_bound_comp_as Hcmp.
-  unfold elab_rule in Hcmp.
-  store_bound_comp_as_in Hcmp0 Hcmp.
-  unfold elab_ctx in Hcmp0.
-  unfold elab_sort.
-  cbv match beta.
-  match goal with
-    [|- context ctx [named_list_lookup_err
-                       (nth_tail ?n ?l) ?s]] =>
-    let r := eval compute in (named_list_lookup_err
-                                (nth_tail n l) s) in
-    let x := context ctx [r] in
-    change x; cbn
-  end.
-  rewrite !monad_bind_ret.
-  process_interactive.
-  simpl.
-  cbn [elab_lang].
-  pose (tst := nth_tail 1 cat_lang).
-  
-  unfold elab_lang.
-  TODO: best way to reduce to first ask?
-  
-  
-  process_interactive.
-
-Derive cat_lang_pf SuchThat (Some cat_lang = synth_wf_lang cat_lang_pf) As cat_lang_pf_ok.
-Proof.
-  assert (elab_lang_structure cat_lang cat_lang_pf) > [ repeat constructor | ].
-  cbn.
-  match! goal with
-  | [|- context c[?s \notin ?l]] =>
-     let e:= Std.eval_vm None constr:($s \notin $l) in
-     change ($c e)
-  end.
-  ltac1:(break_monadic_do).
-  }
-    auto with imcore.
-
-Section InferSub.
-
-  Context (subst_lang_el_ty : ctx -> exp (*G*) -> exp (*e*) -> exp).
-
-  
-  Fixpoint sub_decompose g f : exp :=
-    if f == g then {{e #"id"}}
-    else match f with
-         | con "cmp" [:: h; f'] =>
-           {{e #"cmp" {sub_decompose g f'} {h} }}
-         | _ => {{e #"ERR"}}
-         end.
-
-  (*Only works sometimes; not guaranteed to be correct *)
-  Definition ty_decompose g A :=
-    if g == {{e #"id"}} then A
-    else match A with
-         | con "ty_subst" [:: A; g'] =>
-           {{e #"ty_subst" {sub_decompose g g'} {A} }}
-         | _ => {{e #"ERR: ty_decompose"}}
-         end.
-
-  Fixpoint cat_lang_sub_r c e G_l : exp :=
-    match e with
-    | con "id" [::] => G_l
-    | con "cmp" [:: g; f] =>
-      let G_lf := cat_lang_sub_r c f G_l in
-      let G_lg := cat_lang_sub_r c g G_lf in
-      G_lg
-    | con "wkn" [::] =>
-      match G_l with
-      | con "ext" [:: _;G_r] => G_r
-      | _ => {{e #"ERR"}}
-      end
-    | con "snoc" [:: e; f] =>
-      let G' := cat_lang_sub_r c f G_l in
-      let Af := subst_lang_el_ty c G' e in
-      {{e #"ext" {G'} {ty_decompose f Af} }}
-    | var x =>
-      match named_list_lookup {{s #"ERR"}} c x with
-      | scon "sub" [:: G; _] => G
-      | _ => {{e #"ERR"}}
-      end
-    | _ => {{e #"ERR"}}
-    end.
-
-End InferSub.
-  
-Fixpoint subst_lang_el_ty c G e : exp :=
-  match e,G with
-  | var x,_ => 
-    match named_list_lookup {{s #"ERR not in c"}} c x with
-    | scon "el" [:: t; _] => t
-    | _ => {{e #"ERR sort from c not in subst lang"}}
-    end
-  | con "hd" [::], con "ext" [:: A; G'] =>
-    {{e #"ty_subst" #"wkn" %"A" }}
-  | con "el_subst" [:: e'; g], _ =>
-    let G' := cat_lang_sub_r subst_lang_el_ty c g G in
-    let A := subst_lang_el_ty c G' e' in
-    {{e #"ty_subst" {g} {A} }}
-  | _, _ => {{e #"ERR: not in subst lang" }}
-  end.
-
-Import OptionMonad.
-
-Instance rec_cat_lang : LangRecognize cat_lang :=
-  { le_sort_dec := generic_sort_dec_fuel 10 cat_lang;
-    decide_le_sort := @generic_decide_le_sort 10 cat_lang;
-    term_args_elab c s name t := 
-      match name, t, s with
-      | "id", scon "sub" [:: _; G],_ => do ret [:: G]
-      | "cmp", scon "sub" [:: G3; G1], [:: g; f] =>
-        let G2 := cat_lang_sub_r subst_lang_el_ty c f G1 in
-        do ret [:: g; f; G3; G2; G1]
-      | _,_,_ => do ret s
-      end%string;
-    sort_args_elab c s _ := do ret s
-  }.
-
-Lemma cat_lang_wf : wf_lang cat_lang.
-Proof.
-    apply (decide_wf_lang (fuel:=100));
-    vm_compute; constructor.
+  auto_elab.
+  Unshelve.
+  all: cleanup_auto_elab.
 Qed.
 
 
 Definition subst_lang : lang :=
-   [::[:> "G" : #"env", "A" : #"ty" %"G"
+   [[:> "G" : #"env", "A" : #"ty" %"G"
        ----------------------------------------------- ("snoc_wkn_hd")
        #"id" = #"snoc" #"wkn" #"hd" : #"sub" (#"ext" %"G" %"A") (#"ext" %"G" %"A")
    ];
@@ -658,38 +171,106 @@ Definition subst_lang : lang :=
   [s| "G" : #"env" 
       -----------------------------------------------
       #"ty" "G" srt
-  ]]%arule++cat_lang.
- 
-Instance rec_subst_lang : LangRecognize subst_lang :=
-  {  le_sort_dec := generic_sort_dec_fuel 10 subst_lang;
-    decide_le_sort := @generic_decide_le_sort 10 subst_lang;
-    term_args_elab c s name t := 
-      match name, t, s with
-      | "forget", scon "sub" [:: _; G],_ => do ret [:: G]
-      | "id", scon "sub" [:: _; G],_ => do ret [:: G]
-      | "cmp", scon "sub" [:: G3; G1], [:: g; f] =>
-        let G2 := cat_lang_sub_r subst_lang_el_ty c f G1 in
-        do ret [:: g; f; G3; G2; G1]
-      | "ty_subst", scon "ty" [:: G], [:: A; g] =>
-        let G' := cat_lang_sub_r subst_lang_el_ty c g G in
-        do ret [:: A; g; G'; G]
-      | "el_subst", scon "el" [:: _; G], [:: e; g] =>
-        let G' := cat_lang_sub_r subst_lang_el_ty c g G in
-        let A := subst_lang_el_ty c G' e in
-        do ret [:: e; A; g; G'; G]
-      | "snoc", scon "sub" [:: con "ext" [:: A; G']; G], [:: e; g] =>
-        do ret [:: e; g; A; G'; G]
-      | "wkn", scon "sub" [:: G; con "ext" [:: A; _]], [::] =>
-        do ret [:: A; G]
-      | "hd", scon "el" [:: _; con "ext" [:: A; G]], [::] =>
-        do ret [:: A; G]
-      | _,_,_ => do ret s
-      end%string;
-    sort_args_elab c s _ := do ret s
-  }.
-  
-Lemma subst_lang_wf : wf_lang subst_lang.
+   ]]%arule++cat_lang.
+
+
+Derive subst_lang_elab
+       SuchThat (elab_lang subst_lang subst_lang_elab)
+       As subst_lang_wf.
 Proof.
-    apply (decide_wf_lang (fuel:=100));
-    vm_compute; constructor.
+  match goal with
+  | |- elab_lang ?l ?el =>
+        rewrite (as_nth_tail l); rewrite (as_nth_tail el); break_down_elab_lang
+  end.
+  
+Local Ltac t :=
+  match goal with
+  | [|- fresh _ _ ]=> apply use_compute_fresh; compute; reflexivity
+  | [|- sublist _ _ ]=> apply (use_compute_sublist string_dec); compute; reflexivity
+  | [|- In _ _ ]=> apply named_list_lookup_err_in; compute; reflexivity
+  | [|- len_eq _ _] => econstructor
+  | [|-elab_sort _ _ _ _] => eapply elab_sort_by
+  | [|-elab_ctx _ _ _] => econstructor
+  | [|-elab_args _ _ _ _ _ _] => eapply elab_args_cons_ex' || econstructor
+  | [|-elab_term _ _ _ _ _] => eapply elab_term_conv; [eapply elab_term_var || eapply elab_term_by'|]
+  | [|-wf_term _ _ _ _] => ()
+  | [|-elab_rule _ _ _] => econstructor
+  | [|- _ = _] => compute; reflexivity
+  end.
+
+Local Ltac t' :=
+  match goal with
+  | [|- fresh _ _ ]=> apply use_compute_fresh; compute; reflexivity
+  | [|- sublist _ _ ]=> apply (use_compute_sublist string_dec); compute; reflexivity
+  | [|- In _ _ ]=> apply named_list_lookup_err_in; compute; reflexivity
+  | [|- wf_term _ _ _ _] =>  eapply wf_term_var || eapply wf_term_by'
+  | [|- wf_sort _ _ _] => eapply wf_sort_by
+  | [|-wf_args _ _ _ _] => econstructor
+  | [|- _ = _] => compute; reflexivity
+  end.
+
+solve[ repeat t].
+solve[ repeat t].
+solve[repeat t; apply eq_sort_refl; repeat t'].
+solve[repeat t; apply eq_sort_refl; repeat t'].
+{
+  repeat t.
+  all: try solve[apply eq_sort_refl; repeat t'].
+  2: apply eq_sort_refl; repeat t'.
+  all: repeat t'.
+}
+{
+  repeat t.
+  all: try solve[apply eq_sort_refl; repeat t'].
+  all: repeat t'.
+}
+{
+  repeat t.
+  all: try solve[apply eq_sort_refl; repeat t'].
+  all: repeat t'.
+}
+{
+  repeat t.
+  all: try solve[apply eq_sort_refl; repeat t'].
+  all: repeat t'.
+}
+{
+  repeat t.
+  all: try solve[apply eq_sort_refl; repeat t'].
+  all: repeat t'.
+}
+solve[repeat t; try solve[apply eq_sort_refl; repeat t'];repeat t'].
+solve[repeat t; try solve[apply eq_sort_refl; repeat t'];repeat t'].
+solve[repeat t; try solve[apply eq_sort_refl; repeat t'];repeat t'].
+solve[repeat t; try solve[apply eq_sort_refl; repeat t'];repeat t'].
+
+{
+  repeat t.
+  all: try solve[apply eq_sort_refl; repeat t'].
+  all: repeat t'.
+  simpl.
+  reduce.
+}
+
+  all: try solve[apply eq_sort_refl; repeat t'].  
+
+  t'.
+  apply named_list_lookup_err_in; compute.
+  reflexivity.
+  t'.
+  apply eq_sort_refl; repeat t'.
+  simpl. t'.
+  repeat t; repeat t'.
+solve[ repeat t].
+solve[ repeat t].
+
+all: repeat t.
+all: try solve [t'].
+all: simpl.
+apply eq_sort_refl; admit.
+repeat t.
+eapply elab_term_conv.
+eapply elab_term_var.
+
 Qed.
+
